algebraic theory 4-8 [foxtrot]

theories/foxtrot/examples/algebraic.v
@@ -1,6 +1,6 @@
 (** * Algebraic theory *)
 From clutch.foxtrot Require Import foxtrot.
-From clutch.foxtrot.lib Require Import toss or.
+From clutch.foxtrot.lib Require Import toss or diverge nodet.
 
 Set Default Proof Using "Type*".
 
@@ -77,19 +77,180 @@ Section eq2.
 End eq2.
 
 Section eq3.
+  Variable (e1 e2 e3: expr).
+  Variable (τ: type).
+  Variable (p q r s:nat).
+  Variable (Hineq: p<=q+1).
+  Variable (Hineq': r<=s+1).
+
+  Definition intermediate_prog: expr:=
+      (let: "x" := rand ((#q+#1)*(#s+#1)-#1) in
+      if: ("x" < #p*#r) then e1
+      else
+        if: ("x"-#p*#r<#p*(#s+#1-#r))
+        then e2 else e3)%E.
+  Lemma eq3 :
+    ∅ ⊢ₜ e1 : τ -> ∅ ⊢ₜ e2 : τ -> ∅ ⊢ₜ e3 : τ ->
+              ∅ ⊨ toss p q (toss r s e1 e2) e3 =ctx= toss (p*r) ((q+1)*(s+1)-1) e1 (toss (r*(q+1-p)) ((q+1)*(s+1)-p*r-1) e2 e3): τ.
+  Proof.
+    intros H1 H2 H3.
+    eapply (ctx_equiv_transitive) with (intermediate_prog); rewrite /intermediate_prog.
+    - admit.
+    - admit.
+  Admitted. 
 End eq3.
 
 Section eq4.
+  Variable (e: expr).
+  Variable (τ: type).
+  Lemma eq4 :
+      ∅ ⊢ₜ e : τ -> ∅ ⊨ or e e =ctx= e : τ.
+  Proof.
+    intros H;
+    split;
+      apply (refines_sound (#[foxtrotRΣ])); iIntros;
+      iPoseProof (binary_fundamental.refines_typed _ _ _ H) as "H";
+    iIntros; unfold_rel;
+      iIntros (K j) "Hspec".
+    - wp_apply (wp_or with "[-]").
+      + iSplit; by iApply "H".
+      + by iIntros. 
+    - iMod (tp_or _ _ _ true with "[$]").
+      by iApply "H".
+  Qed. 
 End eq4.
 
 Section eq5.
+  Variable (e1 e2 : expr).
+  Variable (τ: type).
+  Lemma eq5 :
+    ∅ ⊢ₜ e1 : τ -> ∅ ⊢ₜ e2 : τ ->
+              ∅ ⊨ or e1 e2 =ctx= or e2 e1 : τ.
+  Proof.
+    intros H1 H2;
+    split;
+      apply (refines_sound (#[foxtrotRΣ])); iIntros;
+      iPoseProof (binary_fundamental.refines_typed _ _ _ H1) as "H1";
+      iPoseProof (binary_fundamental.refines_typed _ _ _ H2) as "H2";
+    iIntros; unfold_rel;
+      iIntros (K j) "Hspec".
+    - wp_apply (wp_or with "[-]").
+      + iSplit.
+        * iMod (tp_or _ _ _ false with "[$]").
+          by iApply "H1".
+        * iMod (tp_or _ _ _ true with "[$]").
+          by iApply "H2".
+      + simpl. by iIntros.
+    - wp_apply (wp_or with "[-]").
+      + iSplit.
+        * iMod (tp_or _ _ _ false with "[$]").
+          by iApply "H2".
+        * iMod (tp_or _ _ _ true with "[$]").
+          by iApply "H1".
+      + simpl. by iIntros.
+  Qed.     
 End eq5.
 
 Section eq6.
+  Variable (e1 e2 e3: expr).
+  Variable (τ: type).
+
+  Lemma eq6 :
+    ∅ ⊢ₜ e1 : τ -> ∅ ⊢ₜ e2 : τ -> ∅ ⊢ₜ e3 : τ ->
+              ∅ ⊨ or e1 (or e2 e3) =ctx= or (or e1 e2) e3: τ.
+  Proof.
+    intros H1 H2 H3.
+    split;
+      apply (refines_sound (#[foxtrotRΣ])); iIntros;
+      iPoseProof (binary_fundamental.refines_typed _ _ _ H1) as "H1";
+      iPoseProof (binary_fundamental.refines_typed _ _ _ H2) as "H2";
+      iPoseProof (binary_fundamental.refines_typed _ _ _ H3) as "H3"; unfold_rel;
+      iIntros (K j) "Hspec"; wp_apply (wp_or with "[-]"); try iSplit; try wp_apply (wp_or with "[-]"); try iSplit.
+    - iMod (tp_or _ _ _ true with "[$]").
+      iMod (tp_or _ _ _ true with "[$]").
+      by iApply "H1".
+    - iMod (tp_or _ _ _ true with "[$]").
+      iMod (tp_or _ _ _ false with "[$]").
+      by iApply "H2".
+    - iMod (tp_or _ _ _ false with "[$]").
+      by iApply "H3".
+    - by iIntros.
+    - by iIntros.
+    - iMod (tp_or _ _ _ true with "[$]").
+      by iApply "H1".
+    - iMod (tp_or _ _ _ false with "[$]").
+      iMod (tp_or _ _ _ true with "[$]").
+      by iApply "H2".
+    - shelve. 
+    - iMod (tp_or _ _ _ false with "[$]").
+      iMod (tp_or _ _ _ false with "[$]").
+      by iApply "H3".
+    - by iIntros.
+      Unshelve.
+      2:{ by iIntros. }
+  Qed. 
 End eq6.
 
 Section eq7.
+  Variable (e: expr).
+  Variable (τ: type).
+  Lemma eq7 :
+      ∅ ⊢ₜ e : τ -> ∅ ⊨ or e (diverge #()) =ctx= e : τ.
+  Proof.
+    intros H;
+    split;
+      apply (refines_sound (#[foxtrotRΣ])); iIntros;
+      iPoseProof (binary_fundamental.refines_typed _ _ _ H) as "H";
+    iIntros; unfold_rel;
+      iIntros (K j) "Hspec".
+    - wp_apply (wp_or with "[-]").
+      + iSplit; first by iApply "H".
+        wp_apply wp_diverge; first done.
+        by iIntros. 
+      + by iIntros. 
+    - iMod (tp_or _ _ _ true with "[$]").
+      by iApply "H".
+  Qed. 
 End eq7.
 
 Section eq8.
+  Variable (e1 e2 e3: expr).
+  Variable (p q:nat).
+  Variable (τ: type).
+  Lemma eq8:
+    ∅ ⊢ₜ e1 : τ -> ∅ ⊢ₜ e2 : τ -> ∅ ⊢ₜ e3 : τ ->
+              ∅ ⊨ or (toss p q e1 e2) (toss p q e1 e3) ≤ctx≤ toss p q e1 (or e2 e3): τ.
+  Proof.
+    intros H1 H2 H3.
+      apply (refines_sound (#[foxtrotRΣ])); iIntros;
+      iPoseProof (binary_fundamental.refines_typed _ _ _ H1) as "H1";
+      iPoseProof (binary_fundamental.refines_typed _ _ _ H2) as "H2";
+      iPoseProof (binary_fundamental.refines_typed _ _ _ H3) as "H3"; unfold_rel;
+        iIntros (K j) "Hspec".
+      wp_apply (wp_or with "[-]").
+    - iSplit.
+      + rewrite /toss.
+        tp_bind j (rand _)%E.
+        wp_apply (wp_couple_rand_rand with "[$]"); first (simpl; lia).
+        iIntros (?) "(%&Hpsec)".
+        simpl.
+        tp_pures j.
+        wp_pures.
+        case_bool_decide; tp_pures j; wp_pures.
+        * by iApply "H1".
+        * iMod (tp_or _ _ _ true with "[$]").
+          by iApply "H2".
+      + rewrite /toss.
+        tp_bind j (rand _)%E.
+        wp_apply (wp_couple_rand_rand with "[$]"); first (simpl; lia).
+        iIntros (?) "(%&Hpsec)".
+        simpl.
+        tp_pures j.
+        wp_pures.
+        case_bool_decide; tp_pures j; wp_pures.
+        * by iApply "H1".
+        * iMod (tp_or _ _ _ false with "[$]").
+          by iApply "H3".
+    - by iIntros.
+  Qed. 
 End eq8.
