theories/foxtrot/lib/toss.v
@@ -5,8 +5,3 @@ Definition toss (p q: nat) (e1 e2 :expr): expr :=
     if: rand #q<#p
     then e1
     else e2.
-
-Definition toss' α (p q: nat) (e1 e2 :expr): expr :=
-    if: rand(#lbl:α) #q<#p
-    then e1
-    else e2.
